\documentclass{article}
\usepackage{amsmath}
\begin{document}
\begin{eqnarray*}
1 + 2 &=& 3 \\
4 + 5 + 0 &=& 7 + 8 \\
9 + 10 + 11 + 12 &=& 13 + 14 + 15 \\
16 + 17 + 18 + 19 + 20 &=& 21 + 22 + 23 + 24 \\
25 + 26 + 27 + 28 + 29 + 30 &=& 31 + 32 + 33 + 34 + 35 \\
\end{eqnarray*}
\begin{eqnarray*}
(a + b)^2 &=& (a + b)(a + b) \\
&=&(a + b)a + (a + b)b\\ 
&=& a(a + b) + b(a + b) \\
&=& a^2 + ab + ba + b^2 \\
&=& a^2 + 2ab + b^2 \\
\end{eqnarray*}
\begin{eqnarray*}
\tan(\alpha + \beta + \gamma) &=& \frac{\tan(\alpha + \beta)}{1-\tan(\alpha + \beta)\tan\gamma} \\
 &=&\frac{\frac{\tan \alpha+\tan \beta}{1- \tan \alpha \tan \beta}+ \tan \gamma}{1- \left ( \frac{\tan \alpha+ \tan \beta}{1- \tan \alpha \tan \beta} \right) \tan \gamma} \\
 &=& \frac{\tan\alpha+\tan\beta+(1-\tan\alpha\tan\beta)\tan\gamma}{1-\tan\alpha\tan\beta-(\tan\alpha+\tan\beta)\tan\gamma}\\
\end{eqnarray*}
\end{document}
